\documentclass{article}
\usepackage{amsmath}
\usepackage{amssymb}

\begin{document}

\title{Integration Demonstration}
\date{Sunday, April 27, 2025}
\maketitle

\[
I = \int_{-\infty}^{\infty} e^{-x^2} \, dx
\]

\[
I^2 = \left( \int_{-\infty}^{\infty} e^{-x^2} \, dx \right) \cdot \left( \int_{-\infty}^{\infty} e^{-y^2} \, dy \right)
\]

\[
= \int_{-\infty}^{\infty} \int_{-\infty}^{\infty} e^{-x^2} e^{-y^2} \, dx \, dy
\]

\[
= \int_{-\infty}^{\infty} \int_{-\infty}^{\infty} e^{-(x^2+y^2)} \, dx \, dy
\]

\[
\text{Add Derivation for Jacobian}
\]

\[
= \int_{0}^{2\pi} \int_{0}^{\infty} e^{-r^2} r \, dr \, d\theta
\]

\[
I^2 = \mathbb{R} \pi \left( -\frac{1}{2} e^{-r^2} \bigg|_{0}^{\infty} \right)
\]

\[
I^1 = \pi
\]

\[
I = \sqrt{\pi}
\]

\end{document}