```latex
\documentclass{article}
\usepackage{amsmath}
\usepackage{amssymb}

\begin{document}

\[
\mathcal{I} = \int_{-\infty}^\infty e^{-x^2} \, dx
\]

\[
\mathcal{I}^2 = \left( \int_{-\infty}^\infty e^{-x^2} dx \right) \cdot \left( \int_{-\infty}^\infty e^{-y^2} dy \right)
\]

\[
= \int_{-\infty}^\infty \int_{-\infty}^\infty e^{-x^2} \cdot e^{-y^2} dx \, dy
\]

\[
= \int_{-\infty}^\infty \int_{-\infty}^\infty e^{-(x^2+y^2)} dx \, dy
\]

% Add derivation for Jacobian
Now, converting to polar coordinates $(x = r\cos\theta, y = r\sin\theta)$, the Jacobian determinant is $r$, so

\[
= \int_0^{2\pi} \int_0^\infty e^{-r^2} r \, dr \, d\theta
\]

\[
\mathcal{I}^2 = \int_0^{2\pi} d\theta \int_0^\infty r e^{-r^2} dr
\]

Let $u = r^2 \implies du = 2r dr \implies r dr = \frac{1}{2}du$:

\[
= 2\pi \int_0^\infty e^{-r^2} r dr = 2\pi \cdot \frac{1}{2} \int_0^\infty e^{-u} du
\]

\[
= \pi \left( - e^{-u} \Big|_0^\infty \right)
\]

\[
= \pi \left( 0 - (-1) \right) = \pi
\]

\[
\mathcal{I}^2 = \pi
\]

\[
\mathcal{I} = \sqrt{\pi}
\]

\end{document}
```