```latex
\documentclass{article}
\usepackage{amsmath}
\usepackage{amssymb}
\begin{document}

\title{Evaluation of the Gaussian Integral}
\author{}
\date{Sunday, April 27, 2025}
\maketitle

\begin{equation*}
    \bar{I} = \int_{-\infty}^{\infty} e^{-x^2} \, dx
\end{equation*}

\begin{equation*}
    \bar{I}^2 = \int_{-\infty}^{\infty} e^{-x^2} \, dx \cdot \int_{-\infty}^{\infty} e^{-y^2} \, dy
\end{equation*}

\begin{equation*}
    = \iint_{-\infty}^{\infty} e^{-x^2} \cdot e^{-y^2} \, dx \, dy
\end{equation*}

\begin{equation*}
    = \iint_{-\infty}^{\infty} e^{-(x^2 + y^2)} \, dx \, dy
\end{equation*}

% Add Derivation for Jacobian 

Switching to polar coordinates $(r, \theta)$ where $x = r\cos\theta$, $y = r\sin\theta$, and $dx\,dy = r\,dr\,d\theta$:

\begin{equation*}
    \bar{I}^2 = \int_0^{2\pi} \int_0^{\infty} e^{-r^2} r \, dr \, d\theta
\end{equation*}

Evaluating the inner integral:

\begin{equation*}
    \int_0^{\infty} e^{-r^2} r \, dr = \left(-\frac{1}{2} e^{-r^2}\right)\Bigg|_0^{\infty} = \frac{1}{2}
\end{equation*}

Thus,

\begin{equation*}
    \bar{I}^2 = \int_0^{2\pi} \frac{1}{2} \, d\theta = \pi
\end{equation*}

Therefore,

\begin{equation*}
    \bar{I} = \sqrt{\pi}
\end{equation*}

\end{document}
```