\documentclass{article}
\usepackage{amsmath}
\usepackage{amssymb}
\usepackage{geometry}
\geometry{a4paper, margin=1in}

\begin{document}

Sunday, April 27, 2025 \hfill 8:13 PM

\begin{align*}
I &= \int_{-\infty}^{\infty} e^{-x^2} \, dx \\
I^2 &= \left( \int_{-\infty}^{\infty} e^{-x^2} \, dx \right) \left( \int_{-\infty}^{\infty} e^{-y^2} \, dy \right) \\
&= \int_{-\infty}^{\infty} \int_{-\infty}^{\infty} e^{-(x^2 + y^2)} \, dx \, dy \\
&= \iint_{-\infty}^{\infty} e^{-(x^2 + y^2)} \, dx \, dy \\
\text{Add Derivation for Jacobian} \\
&= \int_0^{2\pi} \int_0^{\infty} e^{-r^2} r \, dr \, d\theta \\
&= \left( \int_0^{2\pi} d\theta \right) \left( \int_0^{\infty} r e^{-r^2} \, dr \right) \\
&= 2\pi \times \left[ -\frac{1}{2} e^{-r^2} \right]_0^{\infty} \\
&= 2\pi \times \frac{1}{2} \\
&= \pi
\end{align*}

\end{document}